selSort.dfy
@@ -1,43 +1,10 @@
-predicate sorted(a: array<int>)
-   reads a
-{
-   forall j, k :: 0 <= j < k < a.Length ==> a[j] <= a[k]
-}
+include "commons.dfy"
 
+module SelSort{
 
-method Copy(a: array<int>) returns (b: array<int>) 
-    ensures multiset(a[..]) ==  multiset(b[..])
-    ensures a.Length == b.Length
-{ 
-    b := new int[a.Length];
-    var i := 0;
-    while i < a.Length 
-        decreases a.Length - i
-        invariant a.Length == b.Length
-        invariant 0 <= i <= a.Length
-        invariant forall k :: 0 <= k < i ==> a[k] == b[k]
-    {
-        b[i] := a[i];
-        i := i + 1;
-    }
-    assert a[..] == b[..];
-}
+import opened Commons
 
-method Swap(a: array<int>, i: int, j: int) 
-    modifies a
-    requires 0 <= i < a.Length
-    requires 0 <= j < a.Length
-    // Nothing else is changed besides a[i] and a[j]
-    ensures forall x :: 0 <= x < a.Length && x != i && x!= j ==> a[x] == old(a[x])
-    // a[i] and a[j] are swapped
-    ensures a[j] == old(a[i]) && a[i] == old(a[j])
-{
-    var ai, aj := a[i], a[j];
-    a[i] := aj;
-    a[j] := ai;
-}
-
-method SelectionSort(a: array<int>)
+method selectionSort(a: array<int>)
     modifies a
     ensures multiset(a[..]) ==  multiset(old(a)[..])
     ensures sorted(a)
@@ -71,4 +38,5 @@ method SelectionSort(a: array<int>)
         }
         k := k + 1;
     }
+}
 }
