commons.dfy
@@ -1,0 +1,41 @@
+module Commons {
+
+/* Returns True iff a is sorted */
+predicate sorted(a: array<int>)
+   reads a
+{
+   forall j, k :: 0 <= j < k < a.Length ==> a[j] <= a[k]
+}
+
+method Copy(a: array<int>) returns (b: array<int>) 
+    ensures multiset(a[..]) ==  multiset(b[..])
+    ensures a.Length == b.Length
+{ 
+    b := new int[a.Length];
+    var i := 0;
+    while i < a.Length 
+        decreases a.Length - i
+        invariant a.Length == b.Length
+        invariant 0 <= i <= a.Length
+        invariant forall k :: 0 <= k < i ==> a[k] == b[k]
+    {
+        b[i] := a[i];
+        i := i + 1;
+    }
+    assert a[..] == b[..];
+}
+
+method Swap(a: array<int>, i: int, j: int) 
+    modifies a
+    requires 0 <= i < a.Length
+    requires 0 <= j < a.Length
+    // Nothing else is changed besides a[i] and a[j]
+    ensures forall x :: 0 <= x < a.Length && x != i && x!= j ==> a[x] == old(a[x])
+    // a[i] and a[j] are swapped
+    ensures a[j] == old(a[i]) && a[i] == old(a[j])
+{
+    var ai, aj := a[i], a[j];
+    a[i] := aj;
+    a[j] := ai;
+}
+}
