main.dfy
@@ -1,0 +1,49 @@
+include "mergeSort.dfy"
+include "selSort.dfy"
+
+module Sort {
+  import opened MergeSort
+  import opened SelSort
+
+method Main()
+{
+    print "Running MergeSort\n";
+    var a := new int[3];
+    a[0], a[1], a[2] := 8, 6, 4;
+    print "The sorted version of ";
+    print a;
+    print " is ";
+    var a_sorted := mergeSort(a);
+    print a_sorted;
+    print "\n";
+    
+    var b := new int[10];
+    b[0], b[1], b[2], b[3], b[4], b[5], b[6], b[7], b[8], b[9] := 8, 6, 4, 2, 19, 54, 16, 5, 28, 37;
+    print "The sorted version of ";
+    print b;
+    print " is ";
+    var b_sorted := mergeSort(b);
+    print b_sorted;
+    print "\n";
+
+    print "Running SelectionSort\n";
+    print "Running MergeSort\n";
+    var c := new int[3];
+    c[0], c[1], c[2] := 8, 6, 4;
+    print "The sorted version of ";
+    print c;
+    print " is ";
+    selectionSort(c);
+    print c;
+    print "\n";
+    
+    var d := new int[10];
+    d[0], d[1], d[2], d[3], d[4], d[5], d[6], d[7], d[8], d[9] := 8, 6, 4, 2, 19, 54, 16, 5, 28, 37;
+    print "The sorted version of ";
+    print d;
+    print " is ";
+    selectionSort(d);
+    print d;
+    print "\n";
+}
+}
